src/Term.v
@@ -556,6 +556,72 @@ Inductive events: AnnoTerm -> Plc -> Evidence -> Ev -> Prop :=
              (joinp i (*(xi')*) yi' (yi') p) *) .
 Hint Constructors events : core.
 
+Inductive EvSubT: Evidence -> Evidence -> Prop :=
+| evsub_refl_t : forall e : Evidence, EvSubT e e
+| uuSubT: forall e e' i tid l tpl,
+    EvSubT e e' ->
+    EvSubT e (uu i l tpl tid e')
+| ggSubT: forall e e' p,
+    EvSubT e e' ->
+    EvSubT e (gg p e')
+| nnSubT: forall e e' i,
+    EvSubT e e' ->
+    EvSubT e (nn i e').
+
+Inductive req_evidence: AnnoTerm -> Plc -> Evidence -> Plc -> Evidence -> Prop :=
+| is_req_evidence: forall annt t pp p q i e e' es,
+    EvSubT es e ->
+    events annt pp e' (req i p q t e) ->
+    req_evidence annt pp e' q es.
+
+
+(* priv_pol p e --> allow place p to receive evidence with shape e *)
+Definition priv_pol := Plc -> Evidence -> Prop.
+
+Check priv_pol.
+
+Definition satisfies_policy (t:AnnoTerm) (pp:Plc) (ee:Evidence)
+           (q:Plc) (es:Evidence) (pol:priv_pol) :=
+  req_evidence t pp ee q es -> (pol q es).
+
+Definition test_term: Term := att 1 (asp CPY).
+Definition test_term_anno := annotated test_term.
+Compute test_term_anno.
+
+Definition test_init_evidence := uu 1 [] 42 442 mt.
+Definition test_init_evidence2 := uu 2 [] 42 442 mt.
+
+Definition test_pol (p:Plc) (e:Evidence) :=
+  match (p,e) with
+  | (1, (uu 1 [] 42 442 mt)) => False
+  | _ => True
+  end.
+    
+    
+
+Example test_term_satisfies_test_pol: forall pp ee q,
+    satisfies_policy test_term_anno pp ee q mt test_pol.
+Proof.
+  intros.
+  cbn.
+  unfold test_init_evidence.
+  unfold satisfies_policy.
+  intros.
+  unfold test_pol.
+  cbv.
+  intros.
+  invc H.
+  inv H1.
+  auto.
+  invc H1.
+  auto.
+  solve_by_inversion.
+Qed.
+
+
+
+
+
 (*
 Lemma events_range_r:
   forall t v p,
